Added liter function, and proved specs for br and del sort clients

theories/examples/sort_br_del.v
@@ -1,8 +1,8 @@
 (** This file provides three wrappers around the distributed version of merge
 sort, demonstrating Actris's support for delegation and branching:
 
-- [sort_service_br]: a service that allows one to sort a series of lists in 
-  sequence. 
+- [sort_service_br]: a service that allows one to sort a series of lists in
+  sequence.
 - [sort_service_del]: a service that allows one to sort a series of lists in
   parallel by delegating a sort service for a single list to a new channel.
 - [sort_service_br_del]: a service that allows one to sort a series of list by
@@ -17,11 +17,28 @@ Definition sort_service_br : val :=
     sort_service "cmp" "c";;
     "go" "cmp" "c".
 
+Definition sort_client_br : val :=
+  λ: "cmp" "l",
+    let: "c" := start_chan (λ: "c", sort_service_br "cmp" "c") in
+    liter (λ: "l'", send "c" #true;; send "c" "l'";; recv "c") "l";;
+    send "c" #false.
+
 Definition sort_service_del : val :=
   rec: "go" "cmp" "c" :=
     if: ~recv "c" then #() else
     send "c" (start_chan (λ: "c", sort_service "cmp" "c"));;
     "go" "cmp" "c".
+
+Definition sort_client_del : val :=
+  λ: "cmp" "l",
+    let: "c" := start_chan (λ: "c", sort_service_del "cmp" "c") in
+    let: "k" := lnil #() in
+    liter (λ: "l'", send "c" #true;;
+                    let: "c'" := recv "c" in
+                    send "c'" "l'";;
+                    lcons "c'" "k") "l";;
+    send "c" #false;;
+    liter (λ: "c", #();; recv "c") "k".
 
 Definition sort_service_br_del : val :=
   rec: "go" "cmp" "c" :=
@@ -59,6 +76,57 @@ Section sort_service_br_del.
     by iApply "HΨ".
   Qed.
 
+  Definition lllist (I : A → val → iProp Σ)
+             (l : loc) (yys : list (list A)) : iProp Σ :=
+    llist (λ ys l, ∃ (l' : loc), ⌜#l' = l⌝ ∗ llist I l' ys)%I l yys.
+
+  Lemma sort_client_br_spec cmp l xxs :
+    cmp_spec I R cmp -∗
+    {{{ lllist I l xxs }}}
+      sort_client_br cmp #l
+    {{{ yys, RET #(); lllist I l yys ∗
+                       ([∗list] k↦xs;ys ∈ xxs; yys, ⌜Sorted R ys⌝ ∗ ⌜ys ≡ₚ xs⌝) }}}.
+  Proof.
+    iIntros "#Hcmp !>" (Φ) "Hl HΦ". wp_lam.
+    wp_smart_apply (start_chan_spec sort_protocol_br); iIntros (c) "Hc".
+    - wp_lam. iApply (sort_service_br_spec with "[$] Hc"). by iIntros "!> Hc".
+    - wp_smart_apply (liter_spec _ l xxs
+        (λ xs l, ∃ (l' : loc), ⌜#l' = l⌝ ∗ llist I l' xs)%I
+        (λ xs l, ∃ (ys : list A) (l' : loc), ⌜Sorted R ys⌝ ∗ ⌜ys ≡ₚ xs⌝ ∗
+                      ⌜#l' = l⌝ ∗ llist I l' ys)%I
+        (λ _, c ↣ sort_protocol_br)
+                        with "[] [$Hl $Hc]").
+      { iIntros (_ x v) "!>".
+        iIntros (Ψ) "[Hl' Hc] HΨ".
+        iDestruct "Hl'" as (l' <-) "Hl'". wp_lam. wp_select.
+        wp_send with "[Hl'//]".
+        wp_recv (ys) as "[Hsorted [Hperm Hys]]".
+        iIntros "!>".
+        rewrite iProto_app_end_l.
+        iApply "HΨ".
+        iFrame "Hc".
+        iExists ys, l'. by iFrame. }
+      iIntros "[Hl Hc]". wp_pures. wp_select.
+      iDestruct (llist_out with "Hl") as (vs) "[Hvs Hxxs]".
+      iAssert (∃ yys : list (list A),
+                  ([∗ list] x;ys ∈ xxs;yys,
+                            ⌜Sorted R ys⌝ ∗ ⌜ys ≡ₚ x⌝) ∗
+                   [∗ list] ys;v ∈ yys;vs, ∃ (l' : loc),
+                                           ⌜#l' = v⌝ ∗ llist I l' ys)%I
+              with "[Hxxs]" as (yys) "[Hyys Hvs']".
+      { iInduction xxs as [|xs xxs] "IH" forall (vs).
+        - iDestruct (big_sepL2_nil_inv_l with "Hxxs") as %->. eauto.
+        - iDestruct (big_sepL2_cons_inv_l with "Hxxs") as (v vs' ->) "[Hv Hxxs]".
+          iDestruct "Hv" as (ys l' Hsorted Hperm <-) "Hv".
+          iDestruct ("IH" with "Hxxs") as (yys) "[Hyys Hvs]".
+          iExists (ys::yys).
+          iFrame "Hyys Hvs".
+          eauto with iFrame. }
+      iApply "HΦ".
+      iIntros "!>". iFrame "Hyys".
+      iApply (llist_in with "[$Hvs $Hvs']").
+  Qed.
+
   Definition sort_protocol_del_aux (rec : iProto Σ) : iProto Σ :=
     ((<? c> MSG c {{ c ↣ sort_protocol I R }}; rec) <+> END)%proto.
   Instance sort_protocol_del_aux_contractive : Contractive sort_protocol_del_aux.
@@ -68,7 +136,7 @@ Section sort_service_br_del.
     ProtoUnfold sort_protocol_del (sort_protocol_del_aux sort_protocol_del).
   Proof. apply proto_unfold_eq, (fixpoint_unfold sort_protocol_del_aux). Qed.
 
-  Lemma sort_protocol_del_spec cmp c :
+  Lemma sort_service_del_spec cmp c :
     cmp_spec I R cmp -∗
     {{{ c ↣ iProto_dual sort_protocol_del }}}
       sort_service_del cmp c
@@ -80,6 +148,112 @@ Section sort_service_br_del.
       { wp_pures. wp_smart_apply (sort_service_spec with "Hcmp Hc'"); auto. }
       wp_send with "[$Hc']". by wp_smart_apply ("IH" with "Hc"). }
     by iApply "HΨ".
+  Qed.
+
+  Lemma sort_client_del_spec cmp l xxs :
+    cmp_spec I R cmp -∗
+    {{{ lllist I l xxs }}}
+      sort_client_del cmp #l
+    {{{ yys, RET #(); lllist I l yys ∗
+                       ([∗list] k↦xs;ys ∈ xxs; yys, ⌜Sorted R ys⌝ ∗ ⌜ys ≡ₚ xs⌝) }}}.
+  Proof.
+    iIntros "#Hcmp !>" (Φ) "Hl HΦ". wp_lam.
+    wp_smart_apply (start_chan_spec sort_protocol_del); iIntros (c) "Hc".
+    - wp_lam. iApply (sort_service_del_spec with "[$] Hc"). eauto.
+    - wp_smart_apply (lnil_spec with "[//]").
+      iIntros (k) "Hk".
+      iDestruct (llist_unfold_vals with "Hl") as (vs Hlen) "Hl".
+      wp_smart_apply (liter_spec _ l (zip vs xxs)
+        (λ xs l, ⌜xs.1 = l⌝ ∗ ∃ (l' : loc), ⌜#l' = l⌝ ∗ llist I l' xs.2)%I
+        (λ xs l, ⌜xs.1 = l⌝)%I
+        (λ xxs, c ↣ sort_protocol_del ∗
+                  llist (λ xs c,
+                         ∃ (l' : loc), ⌜#l' = xs.1⌝ ∗
+                                       c ↣ <? (xs' : list A)> MSG #()
+                                            {{ ⌜ Sorted R xs' ⌝ ∗ ⌜ xs' ≡ₚ xs.2 ⌝ ∗
+                                               llist I l' xs' }};
+                                       END) k (reverse xxs))%I
+        with "[] [$Hl $Hk $Hc]").
+      { iIntros (xs x v) "!>".
+        iIntros (Ψ) "[H [Hc Hxs]] HΨ".
+        iDestruct "H" as (Heq l' <-) "Hl'". wp_lam. wp_select.
+        wp_recv (c') as "Hc'".
+        wp_send with "[Hl'//]".
+        wp_smart_apply (lcons_spec with "[$Hxs Hc']").
+        { iExists l'. eauto with iFrame. }
+        iIntros "Hxs".
+        iApply "HΨ".
+        rewrite reverse_app.
+        by iFrame. }
+      iIntros "[Hl [Hc Hk]]".
+      iDestruct (llist_fmap (λ (xs : val * list A) (v : val), ⌜xs.1 = v⌝)%I
+                            (λ (xs : val) (v : val), ⌜xs = v⌝)%I fst
+                   with "[] Hl") as "Hl"; [ eauto | ].
+      rewrite fst_zip; [ | lia ].
+      wp_select. iClear "Hc".
+      wp_smart_apply (liter_spec _ k (reverse (zip vs xxs))
+          (λ (xs : val * list A) (c : val),
+              ∃ l' : loc,
+                ⌜#l' = xs.1⌝
+                ∗ c ↣ (<? (xs' : list A)> MSG #() {{ ⌜Sorted R xs'⌝
+                                                     ∗ ⌜xs' ≡ₚ xs.2⌝ ∗
+                                                       llist I l' xs' }}; END))%I
+          (λ (xs : val * list A) (v : val),
+           ∃ (l' : loc) xs',
+             ⌜#l' = xs.1⌝ ∗ ⌜Sorted R xs'⌝ ∗ ⌜xs' ≡ₚ xs.2⌝ ∗ llist I l' xs')%I
+          (λ _, True)%I with "[] [$Hk]").
+      { iIntros (_ x v) "!>".
+        iIntros (Ψ) "[Hc _] HΨ".
+        iDestruct "Hc" as (l' Heq) "Hc".
+        wp_pures. wp_recv (xs') as "[Hsorted [Hperm Hl']]". iClear "Hc".
+        iIntros "!>".
+        iApply "HΨ".
+        eauto with iFrame. }
+      iIntros "[Hk _]".
+      iDestruct (llist_out with "Hk") as (vs') "[_ Hxxs]".
+      iDestruct (big_sepL2_reverse_2 with "Hxxs") as "Hxxs".
+      rewrite reverse_involutive.
+      iAssert ([∗ list] xs;v ∈ xxs;vs,
+                                   ∃ (l' : loc) (xs' : list A),
+                                     ⌜#l' = v⌝ ∗ ⌜Sorted R xs'⌝ ∗
+                                     ⌜xs' ≡ₚ xs⌝ ∗ llist I l' xs')%I
+        with "[Hxxs]" as "Hxxs".
+      {
+        iRevert (Hlen).
+        generalize (reverse vs'); clear vs'; intros vs'.
+        iInduction xxs as [|xs xxs] "IH" forall (vs vs'); iIntros (Hlen).
+        - by rewrite (nil_length_inv vs); [ | eauto ].
+        - assert (∃ v' vs', vs = v' :: vs') as [v' [vs'' ->]].
+          { destruct vs; eauto.
+            inversion Hlen. }
+          iDestruct (big_sepL2_cons_inv_l with "Hxxs") as (tmp1 tmp2 ->) "Hxxs".
+          iDestruct "Hxxs" as "[Hxs Hxxs]".
+          iDestruct "Hxs" as (l' xs' Heq) "[Hsorted [Hperm Hl']]".
+          iSplitR "Hxxs".
+          { eauto with iFrame. }
+          iApply ("IH" with "Hxxs").
+          eauto.
+      }
+      iAssert (∃ yys : list (list A),
+                    ([∗ list] x;ys ∈ xxs;yys,
+                   ⌜Sorted R ys⌝ ∗ ⌜ys ≡ₚ x⌝) ∗
+                    [∗ list] ys;v ∈ yys;vs, ∃ (l' : loc),
+                    ⌜#l' = v⌝ ∗ llist I l' ys)%I
+                with "[Hxxs]" as (yys) "[Hyys Hvs']".
+      {
+        clear Hlen vs'.
+        iInduction xxs as [|xs xxs] "IH" forall (vs).
+        - iDestruct (big_sepL2_nil_inv_l with "Hxxs") as %->. eauto.
+        - iDestruct (big_sepL2_cons_inv_l with "Hxxs") as (v vs' ->) "[Hv Hxxs]".
+          iDestruct "Hv" as (l' ys <- Hsorted Hperm) "Hl".
+          iDestruct ("IH" with "Hxxs") as (yys) "[Hyys Hvs]".
+          iExists (ys::yys).
+          simpl. iFrame "Hyys Hvs".
+          eauto with iFrame.
+      }
+      iApply "HΦ".
+      iFrame.
+      iApply llist_in. iFrame.
   Qed.
 
   Definition sort_protocol_br_del_aux (rec : iProto Σ) : iProto Σ :=
@@ -108,4 +282,5 @@ Section sort_service_br_del.
       by wp_smart_apply ("IH" with "Hc"). }
     by iApply "HΨ".
   Qed.
+
 End sort_service_br_del.
