theories/utils/llist.v
@@ -86,14 +86,39 @@ Definition lreverse : val :=
   λ: "l", let: "l'" := ref (!"l") in
           "l" <- !(lreverse_at "l'" (lnil #())).
 
+Definition lmap : val :=
+  rec: "go" "f" "l" :=
+  match: !"l" with
+    NONE => "l"
+  | SOME "p" =>
+    let: "x" := "f" (Fst "p") in
+    let: "l'" := "go" "f" (Snd "p") in
+    "l" <- SOME ("x", "l'");; "l"
+  end.
+
+Definition liter : val :=
+  rec: "go" "f" "l" :=
+  match: !"l" with
+    NONE => #()
+  | SOME "p" => "f" (Fst "p");; "go" "f" (Snd "p")
+  end.
+
 Section lists.
-Context `{heapGS Σ} {A} (I : A → val → iProp Σ).
+Context `{heapGS Σ}.
 Implicit Types i : nat.
-Implicit Types xs : list A.
 Implicit Types l : loc.
 Local Arguments llist {_ _ _} _ _ !_ /.
 
-Lemma llist_fmap {B} (J : B → val → iProp Σ) (f : A → B) l xs :
+Lemma cons_length_inv {A : Type} (xs : list A) n :
+  length xs = S n → ∃ x xs', xs = x :: xs'.
+Proof. intros Hlen. destruct xs; [ inversion Hlen | eauto ]. Qed.
+
+Lemma list_app_comm {A} (xs ys zs : list A) :
+  (xs ++ ys) ++ zs = xs ++ (ys ++ zs).
+Proof. induction xs; [ eauto | by simpl; f_equiv ]. Qed.
+
+Lemma llist_fmap {A B} (I : A → val → iProp Σ)
+      (J : B → val → iProp Σ) (f : A → B) l xs :
   □ (∀ x v, I x v -∗ J (f x) v) -∗
   llist I l xs -∗ llist J l (f <$> xs).
 Proof.
@@ -102,11 +127,96 @@ Proof.
   iSplitL "Hx". by iApply "Hf". by iApply "IH".
 Qed.
 
-Lemma lnil_spec :
+Lemma llist_out {A : Type} l (xs : list A) (I : A → val → iProp Σ) :
+  (llist I l xs)%I -∗
+  ∃ vs, (llist (λ x v, ⌜x = v⌝) l vs ∗
+    [∗list] k↦x;v ∈ xs;vs, I x v)%I.
+Proof.
+  iIntros "Hl".
+  iInduction xs as [|x xs] "IH" forall (l).
+  - eauto.
+  - iDestruct "Hl" as (v l') "[HI [Hl Hrec]]".
+    iDestruct ("IH" with "Hrec") as (vs) "[Hxs HIs]".
+    iExists (v::vs).
+    iSplitR "HI HIs"; [ | by iFrame ].
+    iExists v, l'.
+    iSplit; [ done | ].
+    by iFrame "Hl".
+Qed.
+
+Lemma llist_in {A : Type} l (xs : list A) (vs : list val) (I : A → val → iProp Σ) :
+  (llist (λ x v, ⌜x = v⌝) l vs ∗
+    [∗list] k↦x;v ∈ xs;vs, I x v)%I -∗
+  (llist I l xs)%I.
+Proof.
+  iIntros "[Hl HIs]".
+  iInduction xs as [|x xs] "IH" forall (l vs).
+  - by iDestruct (big_sepL2_nil_inv_l with "HIs") as %->.
+  - iDestruct (big_sepL2_cons_inv_l with "HIs") as (v vs' ->) "HIs".
+    iDestruct "Hl" as (v' l' Hv) "[Hl Hrec]".
+    iDestruct "HIs" as "[HI HIs]".
+    iDestruct ("IH" with "Hrec HIs") as "Hxs".
+    iExists v, l'.
+    rewrite Hv.
+    by iFrame "HI Hl".
+Qed.
+
+Lemma llist_unfold_vals {A : Type} l (xs : list A) (I : A → val → iProp Σ) :
+  (llist I l xs)%I -∗
+  ∃ vs, ⌜length vs = length xs⌝ ∗ (llist (λ x v, ⌜x.1 = v⌝ ∗ I x.2 v) l (zip vs xs)).
+Proof.
+  iIntros "Hl".
+  iInduction xs as [|x xs] "IH" forall (l).
+  - iExists []. eauto.
+  - iDestruct "Hl" as (v l') "[HI [Hl Hrec]]".
+    iDestruct ("IH" with "Hrec") as (vs Hlen) "HIs".
+    iExists (v::vs).
+    iSplit.
+    { iPureIntro. simpl. by rewrite Hlen. }
+    iExists v, l'.
+    by iFrame.
+Qed.
+
+Lemma llist_fold_vals {A : Type} l (xs : list A) (I : A → val → iProp Σ) vs :
+  length vs = length xs →
+  (llist (λ x v, ⌜x.1 = v⌝ ∗ I x.2 v) l (zip vs xs)) -∗
+  (llist I l xs)%I.
+Proof.
+  iIntros (Hlen) "Hl".
+  iRevert (Hlen).
+  iInduction xs as [|x xs] "IH" forall (l vs); iIntros (Hlen).
+  - by rewrite (nil_length_inv vs).
+  - destruct (cons_length_inv vs _ Hlen) as [v [vs' ->]].
+    iDestruct "Hl" as (v' l') "[HI [Hl Hrec]]".
+    iDestruct ("IH" with "Hrec []") as "HIs"; [ by eauto | ].
+    iDestruct "HI" as (<-) "HI".
+    iExists v, l'.
+    by iFrame.
+Qed.
+
+Lemma llist_exists {A B : Type} l (xs : list A) (P : A → val → B → iProp Σ) :
+  (llist (λ x v, ∃ y : B, P x v y) l xs)%I -∗
+  (∃ ys : list B, llist (λ _ _, True) l xs ∗
+    [∗list] k↦x;y ∈ xs;ys, ∃ v, P x v y)%I.
+Proof.
+  iIntros "Hl".
+  iInduction xs as [|x xs] "IH" forall (l).
+  - iExists []. eauto.
+  - iDestruct "Hl" as (v l') "[HI [Hl Hrec]]".
+    iDestruct "HI" as (y) "HP".
+    iDestruct ("IH" with "Hrec") as (ys) "[Hxs Hys]".
+    iExists (y::ys).
+    iFrame "Hys".
+    iSplitR "HP"; [ | eauto ].
+    iExists v, l'.
+    by iFrame.
+Qed.
+
+Lemma lnil_spec {A} (I : A → val → iProp Σ) :
   {{{ True }}} lnil #() {{{ l, RET #l; llist I l [] }}}.
 Proof. iIntros (Φ _) "HΦ". wp_lam. wp_alloc l. by iApply "HΦ". Qed.
 
-Lemma lcons_spec l x xs v :
+Lemma lcons_spec {A} I l x (xs : list A) v :
   {{{ llist I l xs ∗ I x v }}} lcons v #l {{{ RET #(); llist I l (x :: xs) }}}.
 Proof.
   iIntros (Φ) "[Hll Hx] HΦ". wp_lam. destruct xs as [|x' xs]; simpl; wp_pures.
@@ -115,7 +225,7 @@ Proof.
     wp_load. wp_alloc k. wp_store. iApply "HΦ"; eauto 10 with iFrame.
 Qed.
 
-Lemma lisnil_spec l xs:
+Lemma lisnil_spec {A} I l (xs : list A) :
   {{{ llist I l xs }}}
     lisnil #l
   {{{ RET #(if xs is [] then true else false); llist I l xs }}}.
@@ -127,7 +237,7 @@ Proof.
 Qed.
 
 (** Not the nicest spec, they leaks *)
-Lemma lhead_spec_aux l x xs :
+Lemma lhead_spec_aux {A} I l x (xs : list A) :
   {{{ llist I l (x :: xs) }}}
     lhead #l
   {{{ v (l' : loc), RET v; I x v ∗ l ↦ SOMEV (v,#l') ∗ llist I l' xs }}}.
@@ -135,7 +245,7 @@ Proof.
   iIntros (Φ) "/=". iDestruct 1 as (v l') "(HIx & Hl & Hll)". iIntros "HΦ".
   wp_lam. wp_load; wp_pures. iApply "HΦ"; eauto with iFrame.
 Qed.
-Lemma lpop_spec_aux l l' v xs :
+Lemma lpop_spec_aux {A} I l l' v (xs : list A) :
   {{{ l ↦ SOMEV (v,#l') ∗ llist I l' xs }}} lpop #l {{{ RET v; llist I l xs }}}.
 Proof.
   iIntros (Φ) "[Hl Hll] HΦ".
@@ -145,7 +255,7 @@ Proof.
     wp_load. wp_store. wp_pures. iApply "HΦ"; eauto with iFrame.
 Qed.
 
-Lemma lhead_spec l x xs :
+Lemma lhead_spec {A} I l x (xs : list A) :
   {{{ llist I l (x :: xs) }}}
     lhead #l
   {{{ v, RET v; I x v ∗ (I x v -∗ llist I l (x :: xs)) }}}.
@@ -155,14 +265,14 @@ Proof.
   simpl; eauto with iFrame.
 Qed.
 
-Lemma lpop_spec l x xs :
+Lemma lpop_spec {A} I l x (xs : list A) :
   {{{ llist I l (x :: xs) }}} lpop #l {{{ v, RET v; I x v ∗ llist I l xs }}}.
 Proof.
   iIntros (Φ) "/=". iDestruct 1 as (v l') "(HIx & Hl & Hll)". iIntros "HΦ".
   wp_smart_apply (lpop_spec_aux with "[$]"); iIntros "Hll". iApply "HΦ"; iFrame.
 Qed.
 
-Lemma llookup_spec l i xs x :
+Lemma llookup_spec {A} I l i (xs : list A) x :
   xs !! i = Some x →
   {{{ llist I l xs }}}
     llookup #l #i
@@ -179,7 +289,7 @@ Proof.
     iApply "HΦ". iIntros "{$HIx} HIx". iExists v, l'. iFrame. by iApply "Hll".
 Qed.
 
-Lemma llength_spec l xs :
+Lemma llength_spec {A} I l (xs : list A) :
   {{{ llist I l xs }}} llength #l {{{ RET #(length xs); llist I l xs }}}.
 Proof.
   iIntros (Φ) "Hll HΦ".
@@ -190,7 +300,7 @@ Proof.
     rewrite (Nat2Z.inj_add 1). iApply "HΦ"; eauto with iFrame.
 Qed.
 
-Lemma lapp_spec l1 l2 xs1 xs2 :
+Lemma lapp_spec {A} I l1 l2 (xs1 xs2 : list A) :
   {{{ llist I l1 xs1 ∗ llist I l2 xs2 }}}
     lapp #l1 #l2
   {{{ RET #(); llist I l1 (xs1 ++ xs2) ∗ (∃ v, l2 ↦ v) }}}.
@@ -206,7 +316,7 @@ Proof.
     iApply "HΦ"; eauto with iFrame.
 Qed.
 
-Lemma lprep_spec l1 l2 xs1 xs2 :
+Lemma lprep_spec {A} I l1 l2 (xs1 xs2 : list A) :
   {{{ llist I l1 xs2 ∗ llist I l2 xs1 }}}
     lprep #l1 #l2
   {{{ RET #(); llist I l1 (xs1 ++ xs2) ∗ (∃ v, l2 ↦ v) }}}.
@@ -219,7 +329,7 @@ Proof.
     iApply "HΦ"; iSplitR "Hl2"; eauto with iFrame.
 Qed.
 
-Lemma lsnoc_spec l xs x v :
+Lemma lsnoc_spec {A} I l (xs : list A) x v :
   {{{ llist I l xs ∗ I x v }}} lsnoc #l v {{{ RET #(); llist I l (xs ++ [x]) }}}.
 Proof.
   iIntros (Φ) "[Hll HIx] HΦ".
@@ -229,7 +339,7 @@ Proof.
     wp_smart_apply ("IH" with "Hll HIx"); iIntros "Hll". iApply "HΦ"; eauto with iFrame.
 Qed.
 
-Lemma lsplit_at_spec l xs (n : nat) :
+Lemma lsplit_at_spec {A} I l (xs : list A) (n : nat) :
   {{{ llist I l xs }}}
     lsplit_at #l #n
   {{{ k, RET #k; llist I l (take n xs) ∗ llist I k (drop n xs) }}}.
@@ -246,7 +356,7 @@ Proof.
       iApply "HΦ"; eauto with iFrame.
 Qed.
 
-Lemma lsplit_spec l xs :
+Lemma lsplit_spec {A} I l (xs : list A) :
   {{{ llist I l xs }}}
     lsplit #l
   {{{ k xs1 xs2, RET #k; ⌜ xs = xs1 ++ xs2 ⌝ ∗ llist I l xs1 ∗ llist I k xs2 }}}.
@@ -258,7 +368,7 @@ Proof.
   iApply "HΦ". iFrame. by rewrite take_drop.
 Qed.
 
-Lemma lreverse_at_spec l xs acc ys :
+Lemma lreverse_at_spec {A} I l (xs : list A) acc ys :
   {{{ llist I l xs ∗ llist I acc ys }}}
     lreverse_at #l #acc
   {{{ l', RET #l'; llist I l' (reverse xs ++ ys) }}}.
@@ -273,7 +383,7 @@ Proof.
     rewrite reverse_cons -assoc_L. iApply "Hl''".
 Qed.
 
-Lemma lreverse_spec l xs :
+Lemma lreverse_spec {A} I l (xs : list A) :
   {{{ llist I l xs }}}
     lreverse #l
   {{{ RET #(); llist I l (reverse xs) }}}.
@@ -291,7 +401,7 @@ Proof.
     wp_load. wp_alloc l' as "Hl'".
     wp_smart_apply (lnil_spec with "[//]").
     iIntros (lnil) "Hlnil".
-    wp_smart_apply (lreverse_at_spec _ (x :: xs) with "[Hl' HI Hrec $Hlnil]").
+    wp_smart_apply (lreverse_at_spec _ _ (x :: xs) with "[Hl' HI Hrec $Hlnil]").
     { simpl; eauto with iFrame. }
     iIntros (l'') "Hl''". rewrite right_id_L. destruct (reverse _) as [|y ys].
     + wp_load. wp_store. by iApply "HΦ".
@@ -299,5 +409,82 @@ Proof.
       wp_load. wp_store.
       iApply "HΦ". eauto with iFrame.
 Qed.
+
+Lemma lmap_fmap_spec {A B} (f : A → B) (fv : val) l (xs : list A)
+      (I : A → val → iProp Σ) (J : B → val → iProp Σ) R :
+  (∀ x v, {{{ I x v ∗ R }}} fv v {{{ w, RET w; J (f x) w ∗ R }}})%I -∗
+  {{{ llist I l xs  ∗ R }}}
+    lmap fv #l
+  {{{ RET #l; llist J l (f <$> xs) ∗ R }}}.
+Proof.
+  iIntros "#Hf" (Φ) "!> [Hl HR] HΦ".
+  iInduction xs as [|x xs] "IH" forall (l Φ); simpl; wp_lam.
+  - wp_load. wp_pures. iApply "HΦ". by iFrame.
+  - iDestruct "Hl" as (v lcons) "[HI [Hlcons Hrec]]".
+    wp_load. wp_pures.
+    wp_apply ("Hf" with "[$HI $HR]").
+    iIntros (w) "[HJ HR]". wp_pures.
+    wp_apply ("IH" with "Hrec HR").
+    iIntros "[Hl HR]".
+    wp_pures.
+    wp_store.
+    iIntros "!>".
+    iApply "HΦ".
+    eauto with iFrame.
+Qed.
+
+Lemma lmap_spec {A} (fv : val) l (xs : list A)
+      (I : A → val → iProp Σ) (J : A → val → iProp Σ) R :
+  (∀ x v, {{{ I x v ∗ R }}} fv v {{{ RET v; J x v ∗ R }}})%I -∗
+  {{{ llist I l xs ∗ R }}}
+    lmap fv #l
+  {{{ RET #l; llist J l xs ∗ R }}}.
+Proof.
+  iIntros "#Hf" (Φ) "!> [Hl HR] HΦ".
+  iInduction xs as [|x xs] "IH" forall (l Φ); simpl; wp_lam.
+  - wp_load. wp_pures. iApply "HΦ". by iFrame.
+  - iDestruct "Hl" as (v lcons) "[HI [Hlcons Hrec]]".
+    wp_load. wp_pures.
+    wp_apply ("Hf" with "[$HI $HR]").
+    iIntros "[HJ HR]". wp_pures.
+    wp_apply ("IH" with "Hrec HR").
+    iIntros "[Hl HR]".
+    wp_pures.
+    wp_store.
+    iIntros "!>".
+    iApply "HΦ".
+    iFrame.
+    iExists _, _. iFrame.
+Qed.
+
+Lemma liter_spec_aux {A} (fv : val) l (xs ys : list A)
+      (I : A → val → iProp Σ) (J : A → val → iProp Σ) R :
+  (∀ xs x v, {{{ I x v ∗ R xs }}} fv v {{{ w, RET w; J x v ∗ R (xs ++ [x]) }}})%I -∗
+  {{{ llist I l xs ∗ R ys }}}
+    liter fv #l
+  {{{ RET #(); llist J l xs ∗ R (ys ++ xs) }}}.
+Proof.
+  iIntros "#Hf" (Φ) "!> [Hl HR] HΦ".
+  iInduction xs as [|x xs] "IH" forall (l ys Φ); simpl; wp_lam.
+  - wp_load. wp_pures. iApply "HΦ". rewrite app_nil_r. by iFrame.
+  - iDestruct "Hl" as (v lcons) "[HI [Hlcons Hrec]]".
+    wp_load. wp_pures.
+    wp_apply ("Hf" with "[$HI $HR]").
+    iIntros (w) "[HJ HR]".
+    wp_smart_apply ("IH" with "Hrec HR").
+    iIntros "[Hl HR]".
+    iApply "HΦ".
+    rewrite list_app_comm.
+    iFrame.
+    iExists _, _. iFrame.
+Qed.
+
+Lemma liter_spec {A} (fv : val) l (xs : list A)
+      (I : A → val → iProp Σ) (J : A → val → iProp Σ) R :
+  (∀ xs x v, {{{ I x v ∗ R xs }}} fv v {{{ w, RET w; J x v ∗ R (xs ++ [x]) }}})%I -∗
+  {{{ llist I l xs ∗ R [] }}}
+    liter fv #l
+  {{{ RET #(); llist J l xs ∗ R xs }}}.
+Proof. iApply liter_spec_aux. Qed.
 
 End lists.
